src/Pipit.Sugar.Base.fst
@@ -21,8 +21,8 @@ type state = {
 type m (a: Type) =
   s: state -> (a & state)
 
-type s (t: table) (a: t.ty)  = m (exp t [] (t.ty_sem a))
-type s' (t: table) (a: Type) = m (exp t [] a)
+type s (t: table) (a: t.ty)  = m (exp t [] a)
+type s' (t: table) (a: funty t.ty)  = m (exp_apps t [] a)
 
 type prim (t: table) (ty: funty t.ty) = p: t.prim { t.prim_ty p == ty }
 
@@ -38,24 +38,24 @@ let fresh' (#ty: eqtype) (t: ty): m (C.var t) =
 let fresh (t: table) (ty: t.ty): s t ty =
   (fun s ->
     let (x, s') = fresh' ty s in
-    (XVar x, s'))
+    (XBase (XVar x), s'))
 
-let run (e: s' 't 'a) : exp 't [] 'a =
+let run (#t: table) (#ty: t.ty) (e: s t ty) : exp t [] ty =
   let (a, _) = e { fresh = 0 } in
   a
 
-let run1 (#a: ('t).ty) (f: s 't a -> s' 't 'b) : exp 't [a] 'b =
+let run1 (#t: table) (#a #b: t.ty) (f: s t a -> s t b) : exp t [a] b =
   let (ax, s) = fresh' a { fresh = 0 } in
-  let a       = XVar ax in
+  let a       = XBase (XVar ax) in
   let (b,  s) = f (m_pure a) s in
   close1 b ax
 
-let run2 (#a #b: ('t).ty) (f: s 't a -> s 't b -> s' 't 'c) : exp 't [a; b] 'c =
+let run2 (#a #b #c: ('t).ty) (f: s 't a -> s 't b -> s 't c) : exp 't [a; b] c =
   let s       = { fresh = 0 } in
   let (ax, s) = fresh' a s in
   let (bx, s) = fresh' b s in
-  let a       = XVar ax in
-  let b       = XVar bx in
+  let a       = XBase (XVar ax) in
+  let b       = XBase (XVar bx) in
   let (c,  s) = f (m_pure a) (m_pure b) s in
   close1 (close1 c bx) ax
 
@@ -66,7 +66,7 @@ let let'
     s 't b =
   (fun s ->
     let (xvar, s) = fresh' a s in
-    let evar = XVar xvar in
+    let evar = XBase (XVar xvar) in
     let (e, s) = e s in
     let (e', s) = f (m_pure evar) s in
     (XLet a e (close1 e' xvar), s))
@@ -77,20 +77,9 @@ let rec'
     s 't a =
   (fun s ->
     let (xvar, s) = fresh' a s in
-    let evar = XVar xvar in
+    let evar = XBase (XVar xvar) in
     let (e', s) = f (m_pure evar) s in
     (XMu (close1 e' xvar), s))
-
-let check'
-  (#a: ('t).ty)
-  (name: string)
-  (e: s 't ('t).propty)
-  (f: s 't a):
-    s 't a =
-  (fun s ->
-    let (e, s) = e s in
-    let (f, s) = f s in
-    (XCheck name e f, s))
 
 // XXX: this unit-check is dangerous, the check will disappear if the returned unit isn't mentioned in the result expression.
 // I really want a monadic/effectful interface that collects a list of checks.
@@ -100,10 +89,20 @@ let check
   (name: string)
   (e: s 't ('t).propty):
     s 't ('t).propty =
-  let' e (fun p -> check' name p p)
+  (fun s ->
+    let (e, s) = e s in
+    (XCheck name e, s))
+
+let check'
+  (#a: ('t).ty)
+  (name: string)
+  (e: s 't ('t).propty)
+  (f: s 't a):
+    s 't a =
+  let' (check name e) (fun _ -> f)
 
 let pure (#a: ('t).ty) (v: ('t).ty_sem a): s 't a =
-  m_pure (XVal v)
+  m_pure (XBase (XVal v))
 
 (* followed-by, initialised delay *)
 let fby (#a: ('t).ty) (v: ('t).ty_sem a) (e: s 't a): s 't a = (fun s -> let (e, s) = e s in (XFby v e, s))
@@ -116,55 +115,45 @@ let fby (#a: ('t).ty) (v: ('t).ty_sem a) (e: s 't a): s 't a = (fun s -> let (e,
 let pre (#a: ('t).ty) (e: s 't a): s 't a = fby (('t).val_default a) e
 
 (* "p -> q" in Lustre, first element of p then remainder of q *)
-let (-->) (#a: ('t).ty) (e1 e2: s 't a): s 't a =
-  (fun s ->
-    let (e1, s) = e1 s in
-    let (e2, s) = e2 s in
-    (XThen e1 e2, s))
+// XXX: needs ifthenelse primitive (if (true fby false) then e1 else e2)
+// let (-->) (#a: ('t).ty) (e1 e2: s 't a): s 't a =
+//   (fun s ->
+//     let (e1, s) = e1 s in
+//     let (e2, s) = e2 s in
+//     (XThen e1 e2, s))
 
 // #push-options "--ifuel 0 --fuel 0"
-let (<$>)
-  (#a: ('t).ty)
-  (#b: funty ('t).ty)
-  (f: prim 't (FTFun a b))
-  (e: s 't a):
-      s' 't (funty_sem ('t).ty_sem b) =
-  let sem = ('t).ty_sem in
-  lemma_funty_sem_FTFun ('t).ty_sem a b;
-  (fun s ->
-    let (aa, s) = e s in
-    (XApp (XPrim f) aa, s))
-
-let (<*>)
-  (f: s' 't ('a -> 'b))
-  (e: s' 't 'a):
-      s' 't 'b =
-  (fun s ->
-    let (f, s) = f s in
-    let (a, s) = e s in
-    (XApp f a, s))
 
 let liftP1
   (#a #b: ('t).ty)
   (f: prim 't (FTFun a (FTVal b)))
   (e: s 't a):
       s 't b =
-  f <$> e
+  (fun s ->
+    let (aa, s) = e s in
+    (XApps (XApp (XPrim f) aa), s))
 
 let liftP2
   (#a #b #c: ('t).ty)
   (f: prim 't (FTFun a (FTFun b (FTVal c))))
-  (a': s 't a)
-  (b': s 't b):
+  (ea: s 't a)
+  (eb: s 't b):
        s 't c =
-  f <$> a' <*> b'
+  (fun s ->
+    let (aa, s) = ea s in
+    let (bb, s) = eb s in
+    (XApps (XApp (XApp (XPrim f) aa) bb), s))
 
 let liftP3
   (#a #b #c #d: ('t).ty)
   (f: prim 't (FTFun a (FTFun b (FTFun c (FTVal d)))))
-  (a': s 't a)
-  (b': s 't b)
-  (c': s 't c):
-      s 't d =
-  f <$> a' <*> b' <*> c'
+  (ea: s 't a)
+  (eb: s 't b)
+  (ec: s 't c):
+       s 't d =
+  (fun s ->
+    let (aa, s) = ea s in
+    let (bb, s) = eb s in
+    let (cc, s) = ec s in
+    (XApps (XApp (XApp (XApp (XPrim f) aa) bb) cc), s))
 
